LeanToLambdaBox/ToLambdaBox.lean
@@ -7,6 +7,18 @@ structure NameContext (aliases: TypeAliasContext) (globals: GlobalValueContext) 
   globals: globals.Map GlobalName
   inductives: inductives.Map MutualInductiveName
 
+-- This Inhabited instance should only be necessary while there are still panics for unimplemented bits.
+unseal TypeAliasContext.Map in
+unseal GlobalValueContext in
+unseal GlobalValueContext.Map in
+unseal InductiveContext.Map in
+instance: Inhabited (NameContext aliases globals inductives) where
+  default := {
+    aliases := show Vector _ _ from default,
+    globals := show Vector _ _ from default,
+    inductives := show Vector _ _ from default,
+  }
+
 def NameContext.empty: NameContext .empty .empty .empty where
   aliases := .empty
   globals := .empty
@@ -17,48 +29,63 @@ def expressionToLambdaBox
   (e: TypedML.Expression cfg globals inductives locals)
   (names: NameContext aliases globals inductives)
   (hConstructors: cfg.constructors = .applied)
-  : Except String LBTerm
-  := do
+  : LBTerm
+  :=
   match e with
-  | .box => return .box
-  | .global id => return .const (names.globals.get id)
-  | .local id => return (.bvar id.deBruijnIndex)
+  | .box => .box
+  | .global id => .const (names.globals.get id)
+  | .local id => (.bvar id.deBruijnIndex)
   | .constructorVal h cid => (show False by rewrite [hConstructors] at h; contradiction).elim
-  | .constructorApp h cid args => throw "constructors not yet implemented"
-  | .app f x => return .app (← expressionToLambdaBox f names hConstructors) (← expressionToLambdaBox x names hConstructors)
-  | .lambda name ext body => return .lambda name (← expressionToLambdaBox body names hConstructors)
+  | .constructorApp h cid args => panic! "constructors not yet implemented"
+  | .app f x => .app (expressionToLambdaBox f names hConstructors) (expressionToLambdaBox x names hConstructors)
+  | .lambda name ext body => .lambda name (expressionToLambdaBox body names hConstructors)
 
 unseal ConstructorName in
-def constructorDeclToLambdaBox (decl: TypedML.ConstructorDecl tvars formers arity): ConstructorBody :=
+def constructorDeclToLambdaBox (decl: TypedML.ConstructorDecl tvars aliases inductives arity): ConstructorBody :=
   {
     name := decl.name,
-    nargs := arity,
+    args := panic! "constructors not yet implemented",
+    originalArity := panic! "constructors not yet implemented",
   }
 
 unseal InductiveName in
-def oneInductiveDeclToLambdaBox (decl: TypedML.OneInductiveDecl tvars formers arities): OneInductiveBody :=
+def oneInductiveDeclToLambdaBox (decl: TypedML.OneInductiveDecl tvars aliases inductives arities): OneInductiveBody :=
   { name := decl.name,
-    ctors : List ConstructorBody := decl.constructors.map (fun _ => constructorDeclToLambdaBox) |>.forget,
-    projs : List ProjectionBody := [],
+    typeVars := panic! "inductive types not yet implemented",
+    ctors := decl.constructors.map (fun _ => constructorDeclToLambdaBox) |>.forget,
+    projs := [],
   }
 
 unseal MutualInductiveName in
-def mutualInductiveDeclToLambdaBox (minds: TypedML.MutualInductiveDecl tvars formers arities): Kername × GlobalDecl :=
-  (minds.name, .inductiveDecl { bodies := minds.inductives.map (fun _ => oneInductiveDeclToLambdaBox) |>.forget, npars := minds.npars } )
+def mutualInductiveDeclToLambdaBox (minds: TypedML.MutualInductiveDecl tvars aliases inductives arities): (Kername × Bool) × GlobalDecl :=
+  -- assuming has_deps is always true
+  ((minds.name, true), .inductiveDecl { bodies := minds.inductives.map (fun _ => oneInductiveDeclToLambdaBox) |>.forget, npars := minds.npars } )
+
+def typeToLambdaBox : TypedML.TType tvars aliases inductives -> LBType
+| .erased => .box
+| .unrepresentable => .any
+| .arrow dom codom => .arr (typeToLambdaBox dom) (typeToLambdaBox codom)
+| .typeVar id => .var id.toIndex
+| .typeFormerApp (.inductive _iid) _args => panic! "inductive types not yet implemented"
+| .typeFormerApp (.alias _id) _args => panic! "type aliases not yet implemented"
+
 
 unseal GlobalName in
 def programToLambdaBox
   (p: TypedML.Program cfg aliases globals inductives)
   (hConstructors: cfg.constructors = .applied)
-  : Except String (GlobalDeclarations × NameContext aliases globals inductives)
-  := do
+  : GlobalDeclarations × NameContext aliases globals inductives
+  :=
   match p with
-  | .empty => return ([], .empty)
-  | .valueDecl p name ext val t =>
-    let (decls, names) ← programToLambdaBox p hConstructors;
-    let value ← expressionToLambdaBox val names hConstructors;
-    return ((name, .constantDecl ⟨.some value⟩) :: decls, { names with globals := names.globals.extend name ext })
-  | .typeAlias _p _name ext tvarnames t => throw "type aliases not yet implemented"
+  | .empty => ([], .empty)
+  | .valueDecl p name ext val t (tvars := tvars) =>
+    let (decls, names) := programToLambdaBox p hConstructors;
+    let value := expressionToLambdaBox val names hConstructors;
+    -- TODO: use real names for type variables somewhere
+    let decl := .constantDecl { body := .some value, type := (List.replicate tvars.size .anon , typeToLambdaBox t)};
+    -- assuming has_deps is always true
+    (((name, true), decl) :: decls, { names with globals := names.globals.extend name ext })
+  | .typeAlias _p _name ext tvarnames t => panic! "type aliases not yet implemented"
   | .mutualInductiveDecl p ext minds =>
-    let (decls, names) ← programToLambdaBox p hConstructors;
-    return ((mutualInductiveDeclToLambdaBox minds) :: decls, { names with inductives := names.inductives.extend minds.name ext })
+    let (decls, names) := programToLambdaBox p hConstructors;
+    (mutualInductiveDeclToLambdaBox minds :: decls, { names with inductives := names.inductives.extend minds.name ext })
